Common/Parser.lean
@@ -1,0 +1,91 @@
+-- import Batteries
+import Std.Internal.Parsec
+
+namespace ParserLib
+open Lean
+open Std.Internal
+open Std.Internal.Parsec
+open Std.Internal.Parsec.String
+
+variable {α β : Type}
+
+/-- end of line -/
+def eol : Parser Unit := pchar '\n' *> return ()
+
+def sepBy1 (p : Parser α) (s : Parser β) : Parser (Array α) := do
+  manyCore (attempt (s *> p)) #[←p]
+
+def endBy (p : Parser α) (e : Parser β) : Parser (Array α) := do
+  manyCore (attempt p) #[←p] <* e
+
+/-- a sequence of space or TAB -/
+def whitespaces : Parser Unit :=
+  many1 (pchar ' ' <|> pchar '\t') *> return ()
+
+/-- an optional sequence of space or TAB -/
+def whitespaces? : Parser Unit :=
+  many (pchar ' ' <|> pchar '\t') *> return ()
+
+/-- a sequence of space, TAB or newline -/
+def delimiter : Parser Unit :=
+  many1 (pchar ' ' <|> pchar '\t' <|> pchar '\n') *> return ()
+
+/-- an optional sequence of space, TAB or newline -/
+def delimiter? : Parser Unit :=
+  many (pchar ' ' <|> pchar '\t' <|> pchar '\n') *> return ()
+
+/-- [A-Za-z]+ -/
+def alphabets := many1Chars asciiLetter
+
+def separator (ch : Char)  : Parser Unit := many1 (pchar ch) *> return ()
+
+def separator₀ (ch : Char)  : Parser Unit := optional (many (pchar ch)) *> return ()
+
+/-- a `Nat` -/
+def number := do
+  let s ← many1 digit
+  return (Array.foldl (fun n (c : Char) => n * 10 + c.toNat - '0'.toNat) (0 : Nat) s)
+
+-- #eval Parsec.run number "21, 8,"
+
+/-- a signed number -/
+def number_p := do
+  let s ← many1 digit
+  return Int.ofNat (Array.foldl (fun n (c : Char) => n * 10 + c.toNat - '0'.toNat) (0 : Nat) s)
+
+def number_m := do
+  let n ← pchar '-' *> number_p
+  return -n
+
+def number_signed := number_m <|> number_p
+
+-- #eval Parser.run number_signed "-21, 8,"
+
+/-- single digit number -/
+def single_digit := (·.toNat - '0'.toNat) <$> digit
+-- #eval Parser.run single_digit "456"
+
+namespace test
+
+def label := many1Chars asciiLetter <* pchar ':'
+
+-- #eval Parsec.run label "Game: 0, "
+
+def fields := sepBy1 (separator₀ ' ' *> label *> separator ' ' *> number) (pchar ',')
+
+-- #eval Parsec.run fields "a: 0, bb: 8"
+
+def parse := pstring "Game:" *> manyChars (pchar ' ') *> digit
+
+-- #eval Lean.Parsec.run parse "Game: 0, "
+
+def parsed (_source : String) : Nat := 0
+
+end test
+
+def parse (parser : Parser α) (source : String) : Option α :=
+  match Parser.run parser source with
+  | Except.ok r    => some r
+  | Except.error _ => none
+
+end ParserLib
