Test/Graph.lean
@@ -37,6 +37,24 @@ def g3 : Graph := {
   root := Fin.ofNat' 7 2,
   filled := by exact Nat.instNeZeroSucc
 }
+
+def independent : Graph := ↑(TreeNode.ofString
+  "{ 1
+    { 2
+      { 3
+        {4 {5 {6 T T} {6 T F}} {5 {6 T T} {6 F F}}}
+        {4 {5 {6 T T} {6 T F}} {5 {6 F F} {6 F F}}} }
+      { 3
+        {4 {5 {6 T T} {6 T F}} {5 {6 T T} {6 F F}}}
+        {4 {5 {6 F F} {6 F F}} {5 {6 F F} {6 F F}}} } }
+    { 2
+      { 3
+        {4 {5 {6 T F} {6 T F}} {5 {6 T F} {6 F F}}}
+        {4 {5 {6 T F} {6 T F}} {5 {6 F F} {6 F F}}} }
+      { 3
+        {4 {5 {6 F F} {6 F F}} {5 {6 F F} {6 F F}}}
+        {4 {5 {6 F F} {6 F F}} {5 {6 F F} {6 F F}}} } } }")
+
 def run : IO Unit := do
   let (start, done) := LogKind.warn.color
   IO.println start
@@ -49,15 +67,21 @@ def run : IO Unit := do
   IO.println s!"g1.compact: {g1.compactNodes.toHashMap.toList}"
   IO.println s!"g2.compact: {g2.compactNodes.toHashMap.toList}"
   IO.println s!"g3.compact: {g3.compactNodes.toHashMap.toList}"
+  IO.println s!"independent.root: {independent.root.val}"
+  IO.println s!"independent: {(independent, independent.root.val)}"
   try
     let gv1 := "lake-test_g2.gv"
     g2.dumpAsDot gv1
-    IO.println =<< IO.Process.run { cmd := "dot", args := #["-T", "png", "-O", gv1]}
+    IO.println gv1 <* IO.Process.run { cmd := "dot", args := #["-T", "png", "-O", gv1]}
     IO.FS.removeFile gv1
     let gv2 := "lake-test_g2-compact.gv"
     g2.compactNodes.dumpAsDot gv2
-    IO.println =<< IO.Process.run { cmd := "dot", args := #["-T", "png", "-O", gv2]}
+    IO.println gv2 <* IO.Process.run { cmd := "dot", args := #["-T", "png", "-O", gv2]}
     IO.FS.removeFile gv2
+    let gv3 := "lake-test_independent.gv"
+    independent.dumpAsDot gv3
+    IO.println gv3 <* IO.Process.run { cmd := "dot", args := #["-T", "png", "-O", gv3]}
+    IO.FS.removeFile gv3
   catch
     | e => IO.println s!"Failed to make a png: {e}"
   IO.println done
