Test/TreeNode.lean
@@ -7,8 +7,27 @@ def t := TreeNode.newConstant true
 def n2 := TreeNode.newVar 2 f t 2 |>.assignIndex |>.fst
 def n3 := TreeNode.newVar 1 f n2 3 |>.assignIndex |>.fst
 
+def independent := TreeNode.ofString
+  "{ 1
+      { 2
+        { 3
+          {4 {5 {6 T T} {6 T F}} {5 {6 T T} {6 F F}}}
+          {4 {5 {6 T T} {6 T F}} {5 {6 F F} {6 F F}}} }
+        { 3
+          {4 {5 {6 T T} {6 T F}} {5 {6 T T} {6 F F}}}
+          {4 {5 {6 F F} {6 F F}} {5 {6 F F} {6 F F}}} } }
+      { 2
+        { 3
+          {4 {5 {6 T F} {6 T F}} {5 {6 T F} {6 F F}}}
+          {4 {5 {6 T F} {6 T F}} {5 {6 F F} {6 F F}}} }
+        { 3
+          {4 {5 {6 F F} {6 F F}} {5 {6 F F} {6 F F}}}
+          {4 {5 {6 F F} {6 F F}} {5 {6 F F} {6 F F}}} } }
+    }"
+
 def test : IO Unit := do
   IO.println "Hello, World!"
   IO.println s!"TreeNode: {f}"
+  IO.println s!"independent: {independent}"
 
 end Test_TreeNode
